SkLean/Typing2.lean
@@ -39,148 +39,33 @@ lemma weakening : valid_judgment_weak e t → valid_judgment e t := by
     apply weakening at h_t_rhs
     exact h_t_rhs
 
-end valid_judgment_weak
+lemma preserved : valid_judgment_weak e t → is_eval_once e e' → valid_judgment_weak e' t := by
+  intro h_t
+  sorry
 
-inductive has_final_judgment : Expr → Expr → Prop
-  | trivial : valid_judgment_weak e t → has_final_judgment e t
-  | hard    : beta_eq t t'            → has_final_judgment e t' → has_final_judgment e t
-
-namespace has_final_judgment
-
-lemma imp_valid_judgment (e : Expr) : has_final_judgment e t → valid_judgment e t := by
-  intro h
-  induction h
-  case trivial _ _ h =>
-    exact h.weakening
-  case hard t' t'' e' h_step h_t' ih =>
-    apply valid_judgment.step_beta_eq
-    exact ih
-    apply beta_eq.symm
-    exact h_step
-
-lemma imp_m : has_final_judgment e t → has_final_judgment e SKM[((M e.max_universe.succ) e)] := by
-  intro h
-  induction h
-  case trivial e' t' h =>
-    apply has_final_judgment.hard
-    apply beta_eq.eval
-    apply is_eval_once.m
-    exact h.weakening
-    exact has_final_judgment.trivial h
-  case hard t' t'' e' h_eval_step h_t' ih =>
-    exact ih
-
-lemma preserved : has_final_judgment e t → is_eval_once e e' → has_final_judgment e' t := by
-  intro h_t h_eval
-  induction h_t
-  case trivial e'' t' h =>
-    cases e'
-    case m m =>
-      match m with
-        | .mk n =>
-          apply has_final_judgment.trivial at h
-          apply has_final_judgment.hard
-          apply beta_eq.symm
-          apply beta_eq.eval
-          apply is_eval_once.m
-          use (Expr.m m).max_universe.succ
-          apply h.imp_valid_judgment
-          apply has_final_judgment.hard
-          apply beta_eq.right
-          apply beta_eq.eval
-          exact h_eval
-          apply has_final_judgment.hard
-          apply beta_eq.eval
-          apply is_eval_once.m
-          apply valid_judgment.m
-          apply has_final_judgment.trivial
-          apply valid_judgment_weak.m
-    case k k =>
-      match k with
-        | .mk n =>
-          apply has_final_judgment.trivial at h
-          apply has_final_judgment.hard
-          apply beta_eq.symm
-          apply beta_eq.eval
-          apply is_eval_once.m
-          use (Expr.k k).max_universe.succ
-          apply h.imp_valid_judgment
-          apply has_final_judgment.hard
-          apply beta_eq.right
-          apply beta_eq.eval
-          exact h_eval
-          apply has_final_judgment.hard
-          apply beta_eq.eval
-          apply is_eval_once.m
-          apply valid_judgment.k
-          apply has_final_judgment.trivial
-          apply valid_judgment_weak.k
-    case s s =>
-      match s with
-        | .mk n =>
-          apply has_final_judgment.trivial at h
-          apply has_final_judgment.hard
-          apply beta_eq.symm
-          apply beta_eq.eval
-          apply is_eval_once.m
-          use (Expr.s s).max_universe.succ
-          apply h.imp_valid_judgment
-          apply has_final_judgment.hard
-          apply beta_eq.right
-          apply beta_eq.eval
-          exact h_eval
-          apply has_final_judgment.hard
-          apply beta_eq.eval
-          apply is_eval_once.m
-          apply valid_judgment.s
-          apply has_final_judgment.trivial
-          apply valid_judgment_weak.s
-    case call c =>
-      match c with
-        | .mk lhs rhs =>
-          cases h
-          cases h_eval
-          cases h_eval
-          cases h_eval
-          case call lhs' rhs' h_u h_t_lhs h_t_rhs =>
-            cases h_t_lhs
-  case hard t'' t''' e' h_beq h_t' ih =>
-    simp_all
-    apply has_final_judgment.hard
-    exact h_beq
-    exact ih
-
-lemma imp_exists_valid_judgment_weak : has_final_judgment e t → ∃ t, valid_judgment_weak e t := by
-  intro h
-  induction h
-  case trivial e' t' h =>
-    use t'
-  case hard t' t'' e' h_eval h_t' ih =>
-    exact ih
-
-end has_final_judgment
-
-namespace valid_judgment
-
-lemma imp_has_final_judgment : valid_judgment e t → has_final_judgment e t := by
-  intro h
-  cases h
-  case k =>
+lemma imp_has_final_judgment_beta_eq : valid_judgment e t₁ → beta_eq t₁ t₂ → has_final_judgment e t₂ := by
+  intro h_t h_eq
+  apply has_final_judgment.hard
+  exact (beta_eq.symm h_eq)
+  cases h_t
+  case a.k =>
     apply has_final_judgment.trivial
     apply valid_judgment_weak.k
-  case s =>
+  case a.s =>
     apply has_final_judgment.trivial
     apply valid_judgment_weak.s
-  case m =>
+  case a.m =>
     apply has_final_judgment.trivial
     apply valid_judgment_weak.m
-  case call lhs rhs h_u h_t_lhs h_t_rhs =>
-    apply has_final_judgment.trivial at h_t_lhs
-    apply has_final_judgment.trivial at h_t_lhs
-    sorry
-  case step_beta_eq t' h_t =>
-    
-    sorry
+  case a.call lhs rhs h_u h_t_lhs h_t_rhs =>
+    apply imp_has_final_judgment_call
+    exact h_u
+    exact h_t_lhs
+    exact h_t_rhs
+  sorry
+termination_by e
+
+end
 
 theorem preserved : valid_judgment e t → is_eval_once e e' → valid_judgment e' t := by
   intro h_t h_eval
